removed extra SpecInstance

Cheriot/CoreConfig.v
@@ -1,4 +1,5 @@
-Require Import Kami.AllNotations ProcKami.Cheriot.Lib ProcKami.Cheriot.Types.
+Require Import Kami.AllNotations.
+Require Import ProcKami.Cheriot.Lib ProcKami.Cheriot.Types ProcKami.Cheriot.InstSpec ProcKami.Cheriot.SpecRun.
 
 Definition CapStruct : Kind :=
   (STRUCT_TYPE {
@@ -228,22 +229,25 @@ Section CapHelpers.
   Definition MtdcValInit := (AddrSz 'h"2000").
 End CapHelpers.
 
-Section Prefix.
-  Variable prefix : string.
-  Variable LgNumMemBytesVal: nat.
-  Variable memInitVal: Fin.t (Nat.pow 2 LgNumMemBytesVal * 8) -> word 8.
-  Definition FullCapWithTagKind := STRUCT_TYPE { "tag" :: Bool;
-                                                 "cap" :: Bit 32;
-                                                 "val" :: Bit 32 }.
-  Variable regsInitVal: Fin.t 32 -> type FullCapWithTagKind.
+Class CoreConfigParams := {
+    prefix : string;
+    LgNumMemBytesVal: nat;
+    memInitVal: Fin.t (Nat.pow 2 LgNumMemBytesVal * 8) -> word 8;
+    FullCapWithTagKind := STRUCT_TYPE { "tag" :: Bool;
+                                        "cap" :: Bit 32;
+                                        "val" :: Bit 32 };
+    regsInitVal: Fin.t 32 -> type FullCapWithTagKind;
+    pcCapInitVal: word 32;
+    pcCapValidThm: PcCapValid capAccessorsInit pcCapInitVal;
+    pcValInitVal: word 32;
+    pcValValidThm: truncLsb pcValInitVal = ZToWord 2 0;
+    hasTrapVal: bool }.
 
-  Variable pcCapInitVal: word 32.
-  Variable pcCapValidThm: PcCapValid capAccessorsInit pcCapInitVal.
-  Variable pcValInitVal: word 32.
-  Variable pcValValidThm: truncLsb pcValInitVal = ZToWord 2 0.
-  Variable hasTrapVal: bool.
+Section Prefix.
+  Context `{coreConfigParams: CoreConfigParams}.
   Lemma pccValidThm: PccValid capAccessorsInit pcCapInitVal pcValInitVal false.
   Proof.
+    destruct coreConfigParams.
     constructor; try intro; auto.
   Qed.
 
@@ -257,7 +261,7 @@ Section Prefix.
       memArrayName := stringify "memArray" n;
       memRfString := stringify "memArrayFile" n |}.
 
-  Definition procParams : ProcParams :=
+  Instance procParams : ProcParams :=
     {|Xlen := 32;
       xlenIs32_or_64 := or_introl eq_refl;
       capAccessors := capAccessorsInit;
@@ -301,4 +305,33 @@ Section Prefix.
       regsRfString := @^"regsArrayFile";
       regsInit := convConstArrayToFunConst regsInitVal;
       hasTrap := hasTrapVal |}.
+
+  Definition getInstEntrySpec (fe: FuncEntry) : list (InstEntry FullOutput) :=
+    map (fun ie => {|instName := instName ie;
+                     uniqId := uniqId ie;
+                     immEncoder := immEncoder ie;
+                     spec := fun ty pcc inst cs1 cs2 scr csr =>
+                               (LETE val <- spec ie pcc inst cs1 cs2 scr csr;
+                                localFunc fe #val)%kami_expr;
+                     instProperties := instProperties ie;
+                     goodInstEncode := goodInstEncode ie;
+                     goodImmEncode := goodImmEncode ie |}) (insts fe).
+
+  Definition specInstEntries := concat (map getInstEntrySpec specFuncUnits).
+
+  Definition specRules : list (forall ty, ActionT ty Void) :=
+    specInstBoundsException ::
+      (fun ty => specInstIllegalException ty specInstEntries) ::
+      map (fun ie ty => specDecExecRule ty scrList csrList ie) specInstEntries.
+
+  Definition specRegs : list RegInitT :=
+    (pcCapReg, existT _ (SyntaxKind (Bit CapSz)) (Some (SyntaxConst pcCapInitVal))) ::
+      (pcValReg, existT _ (SyntaxKind Addr) (Some (SyntaxConst pcValInitVal))) ::
+      (prevPcCapReg, existT _ (SyntaxKind (Bit CapSz)) (Some (SyntaxConst $0))) ::
+      (prevPcValReg, existT _ (SyntaxKind Addr) (Some (SyntaxConst $0))) ::
+      (regsArray, existT _ _ (Some (SyntaxConst (@convTypeToConst (Array 32 FullCapWithTagKind) regsInitVal)))) ::
+      (memArray, existT _ _ (Some (SyntaxConst (@convTypeToConst (Array (NumMemBytes * NumBanks) (Bit 8))
+                                                  memInitVal)))) ::
+      (map (fun x => (regName (scrRegInfo x), existT _ _ (regInit (scrRegInfo x)))) scrList) ++
+      (map (fun x => (regName (csrRegInfo x), existT _ _ (regInit (csrRegInfo x)))) csrList).
 End Prefix.
